\documentclass{amsart}

% PACKAGES

\usepackage{amsmath}
\usepackage{amsfonts}
\usepackage{amssymb,enumerate}
\usepackage{amsthm,stmaryrd}
\usepackage[all]{xy}
\usepackage{hyperref}

%\theoremstyle{definition}
%\newtheorem{exer}{Exercise}

\newcommand{\bbr}{\mathbb{R}}
\newcommand{\bbc}{\mathbb{C}}
\newcommand{\bbz}{\mathbb{Z}}
\newcommand{\bbq}{\mathbb{Q}}
\newcommand{\bbn}{\mathbb{N}}
\newcommand{\be}{\mathbf{e}}
\newcommand{\ba}{\mathbf{a}}
\newcommand{\fm}{\mathfrak{m}}
\newcommand{\Hom}{\operatorname{Hom}}
\renewcommand{\ker}{\operatorname{Ker}}
\newcommand{\im}{\operatorname{Im}}
\newcommand{\xra}{\xrightarrow}
\newcommand{\wti}{\widetilde}

\theoremstyle{plain}
\newtheorem{lem}{Lemma}
\newtheorem{cor}[lem]{Corollary}
\newtheorem{prop}[lem]{Proposition}
\newtheorem{thm}[lem]{Theorem}
\newtheorem{conj}[lem]{Conjecture}
\newtheorem{intthm}{Theorem}
\renewcommand{\theintthm}{\Alph{intthm}}

\theoremstyle{definition}
\newtheorem{defn}[lem]{Definition}
\newtheorem{ex}[lem]{Example}
\newtheorem{question}[lem]{Question}
\newtheorem{questions}[lem]{Questions}
\newtheorem{problem}[lem]{Problem}
\newtheorem{disc}[lem]{Remark}
\newtheorem{rmk}[lem]{Remark}
\newtheorem{construction}[lem]{Construction}
\newtheorem{notn}[lem]{Notation}
\newtheorem{fact}[lem]{Fact}
\newtheorem{para}[lem]{}
\newtheorem{exer}[lem]{Exercise}
\newtheorem{remarkdefinition}[lem]{Remark/Definition}
\newtheorem{notation}[lem]{Notation}
\newtheorem{step}{Step}
\newtheorem{convention}[lem]{Convention}
\newtheorem*{Convention}{Convention}
\newtheorem{assumption}[lem]{Assumption}

\newcommand{\fmn}{F^{m\times n}}
\newcommand{\fnn}{F^{n\times n}}
\newcommand{\col}{\operatorname{Col}}
\newcommand{\row}{\operatorname{Row}}
\newcommand{\Span}{\operatorname{Span}}	
\newcommand{\rank}{\operatorname{rank}}	
\begin{document}

\noindent MATH 8510, Abstract Algebra I \\
Fall 2016\\
Exercises 4-2\\
Due date Thu 15 Sep 4:00PM

\

%\noindent
%Throughout this homework set, let $F$ be a field
%
%
%\


\begin{exer}
Let $A$ and $B$ be groups, and set $A':=\{(a,e_B)\in A\times B\mid a\in A\}\subseteq A\times B$.
\begin{enumerate}[(a)]
\item 
Prove that $A'$ is a normal subgroup of $A\times B$.
\begin{proof}
	$ $\newline
	We show it by the definition of a subgroup.\\
	First we show $A' \leq A \times B$.\\
	Since $A$ is a group, $e_A \in A$.\\
	Then $(e_A,e_B) \in A'$.\\
	So $A' \neq \emptyset$.\\
	$\forall a_1,a_2 \in A, x = (a_1, e_B) \in A',y =  (a_2,e_B) \in A'$,
	\begin{align*}
		xy^{-1} &= (a_1, e_B)(a_2,e_B)^{-1} \\
					  &= (a_1, e_B)({a_2}^{-1},{e_B}^{-1}) \\
					  &= (a_1{a_2}^{-1},e_B{e_B}^{-1}) \\
					  &= (a_1{a_2}^{-1},e_B).
	\end{align*}
	Since $A$ is a group and $a_1,a_2 \in A$, $a_1{a_2}^{-1} \in A$.\\
	So $xy^{-1} = (a_1{a_2}^{-1},e_B) \in A'$.\\
	Besides, $A' \subseteq A\times B$ by the definition of $A'$.\\
	Thus, $A' \leq A \times B$.\\
\end{proof}
\item Prove that $A'\cong A$ and $(A\times B)/A'\cong B$.
	\begin{proof}
		$ $\newline
		\begin{enumerate}[(i)]
		\item
			Define
				\begin{align*}
					f: A& \to A' \\
					a& \mapsto (a,e_B).
				\end{align*}
				$\forall x, y \in A$, 
			\begin{align*}
				f(xy) &= (xy, e_B) \\
				  	  &= (xy,e_Be_B) \\
				  	  &= (x,e_B)(y,e_B) \\
				  	  &= f(x)f(y)
			\end{align*}
			So $f$ is a homomorphism.\\
			Since
				\begin{align*}
					\forall a \in \ker(f) & \Longleftrightarrow f(a) = (e_A,e_B)\\
										  & \Longleftrightarrow (a, e_B) = (e_A,e_B) \\			
										  & \Longleftrightarrow a = e_A,			
				\end{align*}
			$\ker(f) = e_A$.\\
			So $f$ is $1$-$1$.\\
			$\im(f) = \{(a,e_B)| a\in A\} = \{(a,e_B)\in A\times B\mid a\in A\} = A' $ \\ 
			So $f$ is onto.\\
			Thus, $f$ is an isomorphism.\\
			Hence, $A'\cong A$.
		\item 
			Define
				\begin{align*}
					F:  A \times B &\to B\\
							 (a,b) &\mapsto b
				\end{align*}
				$\forall a,b\in A, c,d \in B, ac,bd \in A\times B $, then   
			\begin{align*}
				F\big((a,b)(c,d)\big) &= F\big((ac,bd)\big) \\ 
									  &= bd \\
									  &= F\big((a,b)\big)F\big((c,d)\big).
			\end{align*}
			So $F$ is a homomorphism.\\
			$\forall a \in A, (a,e_B) \in A', F\big((a,e_B)\big) = e_B$.\\
			So $A' \subset \ker(F)$ \\
			Then define
			\begin{align*}
				f: A\times B / A' & \to B. \\
				\overline{(a,b)} & \mapsto F\big((a,b)\big)
			\end{align*}
			Then $f$ is a well-defined homomorphism.\\
			Besides, $\im(f) = \im(F) = \{b | b\in B\} = B$.\\
			So $f$ is onto. \\
			Since
			\begin{align*}
				\forall \overline{(a,b)} \in \ker(f) & \Longleftrightarrow f(\overline{(a,b)}) = e_B\\
													& \Longleftrightarrow F\big((a,b)\big) = e_B \\
													& \Longleftrightarrow b = e_B, a \in A\\
													& \Longleftrightarrow (a,b) \in A', 
			\end{align*}
			$\ker(f) = A'$.\\			
			So $f$ is $1$-$1$.\\
			Thus, $f$ is an isomorphism. \\
			Hence, $(A\times B)/A'\cong B$.

		\end{enumerate}
	\end{proof}
\end{enumerate}
\end{exer}

\begin{exer}
Let $G$ be a group, and consider the commutator subgroup $[G,G]$ from Exercise 4-1.1.
\begin{enumerate}[(a)]
\item Prove that $[G,G]$ is a normal subgroup of $G$.
	\begin{proof}
		$\forall x,y,g \in G, xyx^{-1}y^{-1} \in [G,G]$. \\
		Then 
		\begin{align*}
			g(xyx^{-1}y^{-1})g^{-1} &= gxg^{-1}gyg^{-1}gx^{-1}g^{-1}gy^{-1}g^{-1} \\
     			 		   		  &= (gxg^{-1})(gyg^{-1})(gx^{-1}g^{-1})(gy^{-1}g^{-1}) \\
    	   				  	      &=(gxg^{-1})(gyg^{-1})(gxg^{-1})^{-1}(gyg^{-1})^{-1}.	
		\end{align*}
		Furthermore, $gxg^{-1}, gyg^{-1} \in G$ since $x,y,g \in G$.\\
		So $g(xyx^{-1}y^{-1})g^{-1} \in [G,G]$.\\
		Thus, $[G,G]$ is a normal subgroup of $G$.
	\end{proof}
(Hint: simplify the following product $(gxg^{-1})(gyg^{-1})(gxg^{-1})^{-1}(gyg^{-1})^{-1}$.)
\item Prove that $G/[G,G]$ is abelian.
	\begin{proof}
		$\forall x,y\in G, xyx^{-1}y^{-1} \in [G,G]$.\\
		Then
		    \begin{align*}
		    	 xyx^{-1}y^{-1} \in [G,G] & \Longleftrightarrow xy(yx)^{-1} \in [G,G]\\
		    							  & \Longleftrightarrow xy[G,G] = yx[G,G]\\
		    							  & \Longleftrightarrow x[G,G]y[G,G] = y[G,G]x[G,G]
		    \end{align*}
		since $[G,G]$ is a normal subgroup of $G$.\\
		Thus, $G/[G,G]$ is abelian. 	
	\end{proof}
\item Let $N$ be a normal subgroup of $G$, and prove that $G/N$ is abelian if and only if $[G,G]\subseteq N$.
	\begin{proof}
		$ $\newline
		Since $N$ is a normal subgroup of $G$ and $[G,G] = \{xyx^{-1}y^{-1}|x,y \in G\}$, \\
		$\forall x,y\in G$, 
			\begin{align*}
				G/N \text{ is abelian } &\Longleftrightarrow xNyN = yNxN \\
				 & \Longleftrightarrow xyN = yxN\\
							& \Longleftrightarrow xy(yx)^{-1} \in N \\
				   &\Longleftrightarrow  xyx^{-1}y^{-1} \in N\\
				   &\Longleftrightarrow [G,G]\subseteq N.
			\end{align*}
	\end{proof}
\end{enumerate}
\end{exer}



\end{document}
